---
title: "MATH403: Introduction to Abstract Algebra"
author: Michael Li
geometry: margin=2cm
output: pdf_document
---

# Preliminary Theorems

**Theorem**: $a, c \in Z$ are relatively prime if and only if $\exists x, y \in Z$ such that $ax + cy = 1$

Proof:

- $\implies$ holds by using gcd as a linear combination
- $\impliedby$ if $d \mid a$ and $d \mid c$ then $d \mid ax + cy \implies d \mid 1 \implies d = 1$ so $1$ is the only common factor of $a, b$

# Groups

**Definition**: **Binary Operation** on a set $G$ is a function that assigns each ordered pair of $G$ an element of $G$

$$f: G \times G \rightarrow G$$

**Definition**: A set $G$ is a **Group** is under a binary operation $\circ$ if the following 3 properties are satisfied

1. **Associativity**: $\circ$ is associative so $(\forall a, b, c \in G)[(ab)c = a(bc)]$
2. **Identity**: there is an element $e \in G$ such that $(\forall a \in G)[ae = ea = a]$
3. **Inverses**: $(\forall a \in G)(\exists a^{-1} \in G)[aa^{-1} = a^{-1}a = e]$

**Definition**: A group $G$ is said to be **Abelian** if $(\forall a, b \in G)[ab = ba]$

&nbsp;

**3 Key Properties of Groups**

  - **Uniqueness of Identity**. 

    Proof: Let $(G, \cdot)$ be a group. Suppose by contradiction that $e, e'$ are distinct identities of $G$ then we have

$$e = ee' = e'$$
&nbsp; &nbsp; &nbsp; &nbsp; Which is a contradiction thus $e = e'$

- **Cancellation Property**: $(\forall a, b, c \in G)[ba = c \dot a \implies b = c]$

    Proof: Note that

$$(b \cdot a) \cdot a^{-1} = b = c = (c \cdot a) \cdot a^{-1}$$

- **Each Element Has a Unique Inverse**: $(\forall a \in G)(\exists ! a^{-1} \in G)[aa^{-1} = e = a^{-1}a]$

    Proof: Let $(G, \cdot)$ be a group. Suppose by contradiction that $b, c$ are distinct inverses of $a \in G$. Then we have

$$ab = e = ac$$
&nbsp; &nbsp; &nbsp; &nbsp; However by the cancellation property, $b = c$. Thus we have a contradiction and $a$ has a unique inverse

**Shoes-Socks Property**: $(ab)^{-1} = b^{-1}a^{-1}$

Proof: Note that $(ab)(b^{-1}a^{-1}) = e$

\newpage

**Theorem**: if $a_1, a_2, \ldots, a_n \in G$ then

$$(a_1 \cdots a_n)^{-1} = a_n^{-1} a_{n-1}^{-1} \cdots a_1^{-1}$$

Proof by induction:

- Base case $a_1^{-1} = a_1^{-1}$
- IH: Suppose for an arbitrary $n \geq 1, (a_1 \cdots a_n)^{-1} = a_n^{-1} \cdots a_1^{-1}$
- IS: Let $a = a_1 \cdots a_n$ and $b = a_{n+1}$, then, using the shoes-socks property and IH, we have that

$$(a_1 \cdots a_{n+1})^{-1} = (ab)^{-1} = b^{-1}a^{-1} = a_{n+1}^{-1} \cdots a_1$$

# Subgroups

**Definition**: Let $(G, \cdot)$ be a group, then $H \subseteq G$ is a subgroup if it is closed under $\cdot$ and closed under inverse $(h \in H \implies h^{-1} \in H)$

**Definition**: For any $a \in G$
$$\langle a \rangle = \{a^n \mid n \in Z\}$$ 
is a subgroup called the **cyclic subgroup generated by $a$**

- **Note**: $\langle a \rangle = \langle a^{-1} \rangle$ $\quad (a^{-k} \in \langle a^{-1} \rangle \implies (a^{-k})^{-1} = a^k \in \langle a^{-1} \rangle)$
- **Note**: $\langle 2a \rangle \leq \langle a \rangle$

**Definition**: Let $(G, \cdot)$ be a group. Then

$$Z(G) = \{a \in G \mid (\forall x)[ax = xa]\}$$

is called the **center of $G$**

- **Note**: If $G$ is Abelian, then $Z(G) = G$

**Definition**: Let $(G, \cdot)$ be a group. Then for $a \in G$

$$C(a) = \{x \in G \mid ax = xa\}$$

is the **centralizer** for an element $a \in G$

- **Note**: If $G$ is Abeliean, then $C(a) = G$


&nbsp;

**Theorem**: $Z(G)$ is a subgroup of $G$

Proof: 

- Closure: for arbitrary $a_1, a_2 \in Z(G)$ we have that

$$(a_1a_2)x = a_1a_2x = a_1xa_2 = xa_1a_2 = x(a_1a_2)$$

- Inverse: for $a \in Z(G)$ we have that

$$a^{-1}(ax)a^{-1} = a^{-1}(xa)a^{-1} \implies xa^{-1} = a^{-1} x$$

&nbsp;

**Theorem**: $H, K \leq G \implies H \cap K \leq G$

Proof: use 2 step subgroup test

- $a, b \in H$ and $a, b \in K \implies ab \in H$ and $ab \in K$ by closure $\implies ab \in H \cap K$
- $a, a^{-1} \in H$ and $a, a^{-1} \in K$ by closure of inverses $\implies a, a^{-1} \in H \cap K$

# Cyclic Groups
**Definition**: A group $G$ is **cyclic** if $\exists a \in G$ such that
$$\langle a \rangle = G$$

so all elements are of the form $a^k$. Here $a$ is called the **generator** of $G$

To show that $G$ is cyclic, we need to show

- $G = \langle a \rangle$
- $\langle a \rangle$ has $n$ distinct elements

**Definition**: The **order** $a \in G$ is the least positive exponent $n$ such that $a^n = e$

**Theorem**: For $a \in (G, \cdot)$

- if $|a| = \infty, a^i = a^j$ if and only if $i = j$
- if $|a| = n, a^i = a^j$ if and only if $n \mid i - j$

Proof:

For $|a| = \infty$

- If $i = j$ then clearly $a^i = a^j$
- If $a^i = a^j$ where $i > j$ then for $m > 0$, $i = j +m$ 

$$a^i = a^{j+m} = a^ja^m \implies a^m = e$$
&nbsp; &nbsp; &nbsp; &nbsp; Meaning that $a$ has finite order, which is a contradiction. Thus $a^i \neq a^j$

For $|a| = n$

- If $n \mid i -j \implies a^i = a^j$

    Note that $a^i = a^{j + nk} = a^ja^{nk} = a^j$

- If $a^i = a^j \implies n \mid i -j$

    We have that $a^{i-j} = e$

    If $i =j \rightarrow$ done since $n \mid 0$

    If $i \neq j \rightarrow$ WLOG, $i > j$ then we have

    $i = j + m \implies a^{i-j} = a^m$

    Since $a^i = a^j \implies e = a^m$ so we need to show that $n \mid m$

    We can use Division Algorithm: $\exists! q, r \in Z$ such that $m = nq + r$ for $0 \leq r < n$

    Then we have $a^m = a^{nq + r} = a^r = e \implies r = 0$ since $0 \leq r < n$

    Thus we have shown that $n \mid i -j$

**Corollary** $|a| = |\langle a \rangle|$

**Corollary** $G$ is cyclic $\implies |G| = |a|$

**Corollary** $|a| = n$ and $a^k = e \implies n \mid k$

**Corollary** if $a, b \in G$ have finite order and commute, then $|ab|$ divides lcm$(|a|, |b|)$

Proof: Let $|a| = n, |b| = m, L = \text{lcm}(m, n)$. Then for $r, s \in Z$

$$(ab)^L = a^Lb^L = a^{mr}b^{ns} = e$$

\newpage

**Theorem** $|a| = n \implies |a^k| = \frac{n}{\gcd(n, k)}$ and $\langle a^k \rangle = \langle a^{\gcd(n ,k)} \rangle$

Proof: Let $d = \gcd(n, k)$ and $k = dr$. Then we have

Since $a^k = a^{dr} \implies a^k \in \langle a^d \rangle \implies \langle a^k \rangle \subseteq \langle a^d \rangle$

By gcd as a linear combo, $d = kx + ny$ for $x, y \in Z$. Then

$$a^d = a^{kx + ny} = a^{kx} \implies a^d \in \langle a^k \rangle$$

Thus $\langle a^d \rangle \subseteq \langle a^k \rangle$

Thus $\langle a^d \rangle = \langle a^k \rangle$

&nbsp;

Let $d = \gcd(n, k)$. Clearly, $(a^d)^{n/d} = e$ so we have $|a^d| \leq n/d$

On the other hand, suppose we have $i < n/d$ then $(a^d)^i \neq e$ by the definition of $|a| = n$.

Thus we have $|a^k| = |a^{\gcd(n, k)}| = n/\gcd(n, k)$


**Corollary** if $G$ is cyclic, then the order of any element divides $|G|$

&nbsp;

**Fundamental Theorem of Cyclic Groups**: every subgroup of a cyclic group is cyclic

Proof: Let $H \leq G$

- Case $H = \{e \}$ then $H$ is trivially cyclic
- Case $H \neq \{e \}$ then there is a $b \in H$ such that $b \neq e \implies b = a^k$ for some $k \in Z$

    Furthermore, there must be a $c \in H$ such that $c = a^m$ where $m$ is minimal positive power. Clearly by closure $\langle a^m \rangle \subseteq H$

    Using the division algorithm, we have $k = mq + r \implies a^r = a^{-mq} a ^k \in H$ by closure

    However, $0 \leq r < m$, thus $r = 0$ since $m$ is minimal

    Thus $b = a^k = a^{mq} \in \langle a^m \rangle$

    Thus we have $H = \langle a^m \rangle$


## Ways of Testing Non-Cyclic Group

Use **Countability**: $R$ is uncountable but $\langle a^k \rangle$ is countable. Thus $R$ is not cyclic

Use **Abelian**: Any cyclic group is Abelian but $GL(2, R)$ is not Abelian. Thus $GL(2, R)$ is not cyclic

## Misc Notes

$\langle m \rangle \subseteq \langle d \rangle \implies |m|$ divides $|d|$

$\langle a \rangle \cap \langle b \rangle = \langle lcm(a, b) \rangle$

Smallest subgroup containing $\langle a \rangle$ and $\langle b \rangle$ is $\langle \gcd(a, b) \rangle$

$\langle m, n \rangle = \{mx + ny \mid x, y \in Z\}$ (linear combination of $m$ and $n$)

\newpage


# Permutations

Let $S$ be an arbitrary set. A **permutation** of $S$ is a bijection $S \rightarrow S$.

Then $S_n$, the group of all permutations of $S$ under composition

Important things to note:

- $|S_n| = n!$
- $\epsilon$ is the identity


**Theorem**: every $\sigma \in S_n$ is a product of disjoint cycles

Proof: take $\sigma \in S_n$. 

- If $\sigma = \epsilon = (1) \cdots (n)$ then we are trivially done
- Otherwise start with an arbitrary element $c$ and applying $\sigma(\ldots(\sigma(c)))$ until we get to $\sigma^d(c) = \epsilon$. If this cycles through all possible values, we are done. Otherwise we repeat for the next distinct element

  - **Note**: this works because we know that there are a finite number of values

**Theorem**: order of an $m$-cycle is $m$. Order of a product of multiple disjoint cycles is the lcm of their orders.

  - **Note**: in general $gh = hg \implies |gh| \neq lcm(|g|, |b|)$. Take for example $G = Z_{30}$

    - Let $g = 5 = h \implies |g| = 6 = |h|$. Then $g + h = 10$ but $|g + h| = 3 \neq lcm(|g|, |h|) = 6$. Instead, we showed above that $|gh| \mid lcm(|g|, |h|)$

Proof: Let $|c| = m$, $|d| = n$, $l = lcm(|c|, |d|)$, and $k = |cd|$

We have $(cd)^l = e \implies k \mid l$

Note that if $c, d$ are disjoint then so are $c^k, d^k$. 

Thus we have $(cd)^k = e \implies c^kd^k = e \implies c^k = d^{-k}$

- $d$ fixes all elements of $c$
- $d^k$ fixes all elements of $c$
- $c$ fixes all elements of $d$
- $c^k$ fixes all elements of $d$

Thus $c^k = d^{-k} \implies$ all elements are fixed. 

Thus $c^k = d^{-k} = \epsilon \implies n \mid k, m \mid k \implies l \mid k$

&nbsp;

**Theorem**: for $S_n, n > 1$, any $\sigma \in S_n$ is a product of 2 cycles (may not be disjoint)

Proof: We can take any cycle $c_i$ of order $k$ in $\sigma$ such that $c_i = (a b c \ldots k) = (a k) (a j) \ldots (a b)$. We can repeat this for any cycle in $\sigma$

**Theorem**: $\epsilon = c_1 \ldots c_r$ (all 2 cycles) $\implies r$ is even

Proof by induction:

$r = 1 \implies \epsilon \neq (ab)$ so $r \neq 1$

$r = 2 \implies$ trivially true

IH: For $k < r$, we have that $\epsilon = c_1 \ldots c_k \implies k$ is even

IS: show for $\epsilon = c_1 \ldots c_r$. Take the last 2 cycles. Possible cases are

- $(ab)(ab) = \epsilon$
- $(ab)(bc) = (ac) (ab)$
- $(ac)(cb) = (bc)(ab)$
- $(ab)(cd) = (cd)(ab)$

    Either we get the first case and then by Strong Induction $c_1 \ldots c_{r-2}$ is even or we recurse downard and get the equation $\epsilon = (a?) c_2' \ldots c_r'$. However, the LHS fixes $a$ but the RHS doesn't fix $a$. Thus we have a contradiction and $\epsilon \neq c_1 \ldots c_r$ in the case where $r$ is odd


**Theorem**: If $\sigma \in S_n, n \geq 2$ and $\sigma = c_1 \ldots c_r = f_1 \ldots f_s$ (2 cycles), then $r$ and $f$ have the same parity

Proof: Note that $\sigma \cdot \sigma^{1} = \epsilon$

Then we have $f_s^{-1} \cdots c_{1}^{-1} d_1 \cdots d_r = \epsilon \implies s + r$ is even by previous theorem

Thus either $f, r$ are both odd or $f, r$ are both even

**Definition**: $A_k = \{\sigma \in S_n \mid \sigma \text{ product of even number of 2-cycles}\}$

**Theorem**: $|A_n| = \frac{|S_n|}{2} = \frac{n!}{2}$

Proof: need to show that $|A_n| = |S_n - A_n|$, or that there is a bijection $f: A_n \rightarrow S - A_n$

Take $\sigma \in A_n$ and add a 2-cycle

- $f^{-1}(p) = (1 2) p$
- $f(f^{-1}(p)) = (1 2) (1 2)(p) = p$

Thus there is a bijection and $|A_n| = |S - A_n|$


## Misc Notes

How many elements of order $3$ are in $S_5$?

$|\sigma| = lcm(|c_1|, \ldots)$

So there is a cycle $c_i$ such that $|c_i| = 3$ but we can only have one 3 cycle for any permutation in $S_5$

Thus we can select $5 * 4 * 3/3$ unique 3 cycles, so there are $20$ elements of order $3$ in $S_5$

# Isomorphism

**Definition**: A function $\phi: G \rightarrow G'$ is a **homomorphim** if $\phi(g_1 g_2) = \phi(g'_1) \phi(g'_2)$. If $\phi$ is a bijection, then it is an **isomorphism**

**Properties of Homomorphisms**

- For $e \in G$, $\phi(e) = e' \in G'$. Proof: $\phi(ee) = \phi(e) \phi(e) = \phi(e) \implies e'$ is the identity of $G'$
- For $g \in G$, $\phi(g^{-1}) = (\phi(g))^{-1}$. Proof: $\phi(g g^{-1}) = \phi(e) = \phi(g) \phi(g^{-1}) \implies \phi(g^{-1} = (\phi(g))^{-1}$

**Definition**: **Automorphism** of $G$ is an isomorphic $\phi: G \rightarrow G$

- Trivial example is the identity mapping $\phi(a) = ea = a$ for all $a \in G$
- Aut$(G)$ is the set of all automorphisms of $G$

**Example**: $f: Z_{10} \rightarrow Z_{10}$

- Note that $1$ is a generator of $Z_{10}$ thus $f(1)$ must also be a generator so $f(1) = \{1, 3, 7, 9\} = U(1)$
- Since we are working with addition, $f_a(n) = an$

**Proof**: Aut$(G)$ is a group under function composition

- Given Automorphisms $\phi, \psi$, $\psi\phi$ is also a bijection thus $(\psi \phi)(ab) = \psi(\phi(ab)) = \psi(\phi(a)\phi(b)) = \psi(\phi(a)) \psi(\phi(b)) = (\psi \phi)(a) (\psi \phi)(b)$ is an automorphism and is closed
- Function composition is associative
- The identity mapping $I$ exists where $\phi I = \psi$
- Inverses exists because $\phi$ is bijective

**Proof**: $U(n)$ is isomorphic to Aut$(Z_n)$

**Proof**: Isomorphisms $G \approx H$ are an equivalence relation 

- Reflexivity: Identity mapping $I_G: G \rightarrow G$
- Symmetry: $\phi: G \rightarrow H \implies \phi^{-1}: H \rightarrow G$ by bijection
- Transitivity: $\phi: G \rightarrow H, \psi: H \rightarrow K \implies \psi\phi$ is bijective and is an isomoprhism

**Note**: Aut$(G)$ is a permutation of $G$ but NOT the converse since $|$Aut$(G)|$

**Theorem** $U(n) \approx$ Aut$(Z_n)$

**Note**: $U(p) \approx Z_{p-1}$ where $p$ is a prime since both are cycli of order $p-1$

**Note**: Aut($Z_9)  = (f_1, f_2, f_4, f_5f_7)\approx U(9)$ ????????????????????????????

**Definition**: Inner Automorphism of $G$ is $\phi_a(g) = aga^{-1}$ for $g \in G$

**Proof**: Inn$(G)$ is a group:

- $\phi_a(gg') = aga^{-1}ag'a^{-1} = \phi_a(g)\phi_a(g')$ closure
- $\phi_a(e) = a^{-1} = e$ identity
- 


